protocols/PORExtended.v
@@ -20,6 +20,7 @@ From Coq Require Import
      Classical
      Morphisms
      JMeq
+     Program.Equality
      List.
 
 From KeyManagement Require Import
@@ -48,7 +49,7 @@ From protocols Require Import
      ModelCheck
      ProtocolAutomation
      SafeProtocol
-     LabelsAlign
+     (* LabelsAlign *)
      NoResends
      PartialOrderReduction
 .
@@ -58,7 +59,7 @@ Definition stuck_model_step_user_stuck_user {t__hon t__adv}
   forall uid u,
     (fst st).(users) $? uid = Some u
     -> (forall st', model_step_user uid st st' -> False)
-    -> (forall lbl bd, step_user lbl (Some uid) (build_data_step (fst st) u) bd -> False).
+    -> (forall lbl bd, step_user lbl (Some uid) (build_data_step (fst st) u) bd -> False). 
 
 
 Lemma user_step_label_deterministic :
@@ -79,49 +80,6 @@ Proof.
   invert H.
   invert H6.
 Qed.
-
-(* Lemma user_steps_to_same_place : *)
-(*   forall A B C lbl bd bd1' bd2' suid, *)
-(*     @step_user A B C lbl suid bd bd1' *)
-(*     -> step_user lbl suid bd bd2' *)
-(*     -> bd1' = bd2'. *)
-(* Proof. *)
-(*   induction 1; invert 1; *)
-(*     subst; *)
-(*     eauto. *)
-
-(*   Ltac invertEq := *)
-(*     repeat *)
-(*       match goal with *)
-(*       | [ STEP : step_user ?lbl ?uid (_,_,_,_,_,_,_,_,_,_,Return _) _  |- _] => invert STEP *)
-(*       | [ STEP : step_user ?lbl ?uid ?bd _ , H : (forall _, step_user ?lbl ?uid ?bd _ -> _) |- _] => *)
-(*         apply H in STEP *)
-(*       | [ H : _ = _ |- _ ] => invert H; try contradiction *)
-(*       end. *)
-
-(*   invertEq; eauto. *)
-(*   invertEq; eauto. *)
-(*   invertEq; eauto. *)
-(*   admit. *)
-(*   invertEq; eauto. *)
-(*   invertEq; eauto. *)
-(*   clean_map_lookups; eauto. *)
-(*   clean_map_lookups; eauto. *)
-(*   clean_map_lookups; eauto. *)
-(*   invertEq; eauto. *)
-(*   invertEq; eauto. *)
-
-(*   apply IHstep_user in H7; eauto; invertEq; eauto. *)
-(*   eapply IHstep_user in H7; eauto; invertEq; eauto. *)
-  
-
-  
-(*     repeat *)
-(*       match goal with *)
-(*       | [ H : _ = _ |- _ ] => invert H; try contradiction *)
-(*       end; *)
-(*     eauto. *)
-
 
 Lemma stuck_model_step_user_stuck_user_implies_labels_align :
   forall t__hon t__adv st,
@@ -154,27 +112,37 @@ Qed.
 
 
 Lemma no_model_step_other_user_silent_step :
-  forall t__hon t__adv suid bd bd',
+  forall t t__hon t__adv suid bd bd',
 
     step_user Silent suid bd bd'
     
-    -> forall (usrs usrs' : honest_users t__hon) (adv adv' : user_data t__adv) (cmd cmd' : user_cmd (Base t__hon))
+    -> forall (usrs usrs' : honest_users t__hon) (adv adv' : user_data t__adv) (cmd cmd' : user_cmd t)
         cs cs' gks gks' ks ks' qmsgs qmsgs' mycs mycs' froms froms' sents sents' n n' uid uid' iu,
 
       bd = (usrs,adv,cs,gks,ks,qmsgs,mycs,froms,sents,n,cmd)
       -> bd' = (usrs',adv',cs',gks',ks',qmsgs',mycs',froms',sents',n',cmd')
       -> suid = Some uid
+      -> forall st', model_step_user uid (mkUniverse usrs adv cs gks, iu) st'
       -> uid <> uid'
-      -> (forall st', model_step_user
+      -> forall cmdc ,
+        (forall st', model_step_user
                   uid' 
                   (mkUniverse usrs adv cs gks, iu)
                   st' -> False)
       -> (forall st', model_step_user
                   uid'
-                  (mkUniverse (usrs' $+ (uid, mkUserData ks' cmd' qmsgs' mycs' froms' sents' n'))
+                  (mkUniverse (usrs' $+ (uid, mkUserData ks' cmdc qmsgs' mycs' froms' sents' n'))
                               adv' cs' gks', iu)
                   st' -> False).
 Proof.
+  induct 1; inversion 1; inversion 1; intros; subst; eauto;
+    clean_context.
+
+  - invert H27; unfold build_data_step in *; simpl in *.
+    admit.
+    
+  
+
 Admitted.
 
 Lemma stuck_model_violation_step' :
@@ -202,12 +170,12 @@ Proof.
       rewrite add_neq_o in H1 by auto.
       specialize (H1 _ H5); simpl in H1.
 
-      pose proof (no_model_step_other_user_silent_step
-                    _ _ _ _ _ H6
-                    _ _ _ _ _ _ _ _ _ _ _ _ _ _ _ _ _ _ _ _ _ _ _ _ _
-                    eq_refl eq_refl eq_refl n H3) as NOMODEL.
-      specialize (H1 NOMODEL).
-      eapply H1.
+      (* pose proof (no_model_step_other_user_silent_step *)
+      (*               _ _ _ _ _ H6 *)
+      (*               _ _ _ _ _ _ _ _ _ _ _ _ _ _ _ _ _ _ _ _ _ _ _ _ _ *)
+      (*               eq_refl eq_refl eq_refl n H3) as NOMODEL. *)
+      (* specialize (H1 NOMODEL). *)
+      (* eapply H1. *)
 
       (* Need lemma for :
        *   if I can step now
@@ -216,7 +184,15 @@ Proof.
 
       admit.
 
-  - (* labeled case -- this will perhaps be a bit more difficult because of the ideal world *)
+  (* labeled case -- this will perhaps be a bit more difficult because of the ideal world *)
+  - invert H5.
+    unfold buildUniverse, build_data_step in *; simpl in *.
+
+    destruct (u_id ==n uid); subst; clean_map_lookups.
+    + eapply H3.
+      econstructor 2; eauto.
+    + admit.
+
   
 Admitted.
 
@@ -255,7 +231,7 @@ Module Type SyntacticallySafeProtocol.
   Axiom safe_invariant : invariantFor
                            SYS
                            (fun st => no_resends_U (fst st)
-                                 /\ stuck_step_implies_stuck_universe_step st ).
+                                 /\ stuck_model_step_user_stuck_user st ).
 
 End SyntacticallySafeProtocol.
 
@@ -263,10 +239,10 @@ Module ProtocolSimulates (Proto : SyntacticallySafeProtocol).
   Import Proto.
 
   Lemma no_resends_inv : invariantFor SYS (fun st => no_resends_U (fst st)).
-  Proof. eapply invariant_weaken; [ apply safe_invariant | firstorder idtac]. Qed.
+  Proof. eapply invariant_weaken; [ apply safe_invariant | firstorder idtac ]. Qed.
 
-  Lemma stuck_not_misaligned_inv : invariantFor SYS stuck_step_implies_stuck_universe_step.
-  Proof. eapply invariant_weaken; [ apply safe_invariant | firstorder idtac]. Qed.
+  Lemma stuck_not_misaligned_inv : invariantFor SYS stuck_model_step_user_stuck_user.
+  Proof. eapply invariant_weaken; [ apply safe_invariant | firstorder eauto ]. Qed.
 
   Hint Resolve no_resends_inv stuck_not_misaligned_inv.
 
@@ -532,24 +508,588 @@ Module ProtocolSimulates (Proto : SyntacticallySafeProtocol).
     generalize (reachable_from_labeled_step _ _ _ _ _ H3 STEP LAME H H1 H2);
       intros; split_ex.
 
-    admit.
-    (* pose proof labels_align_inv. *)
-    (* unfold invariantFor, SYS in H5; simpl in H5. *)
-    (* assert ( (ru0,iu0) = (ru0,iu0) \/ False ) as ARG by eauto. *)
-    (* specialize (H5 _ ARG _ H3 _ _ H0). *)
+    pose proof stuck_not_misaligned_inv.
+    unfold invariantFor, SYS in H5; simpl in H5.
+    assert ( (ru0,iu0) = (ru0,iu0) \/ False ) as ARG by eauto.
+    specialize (H5 _ ARG _ H3).
+    apply stuck_model_step_user_stuck_user_implies_labels_align in H5.
 
-    (* split_ex. *)
-    (* do 3 eexists; rewrite H4; repeat apply conj; eauto. *)
-    (* - invert H7; eauto with safe. *)
+    specialize (H5 _ _ H0); split_ex; rewrite H4; (do 3 eexists);
+      repeat simple apply conj; eauto.
+
+    - invert H7; eauto with safe.
       
-    (* - econstructor. *)
+    - econstructor.
 
-    (*   eapply trcEnd_trc. *)
-    (*   generalize (trc_trcEnd H3); intros. *)
-    (*   econstructor; eauto. *)
-    (*   unfold SYS; simpl. *)
-    (*   econstructor; eauto. *)
+      eapply trcEnd_trc.
+      generalize (trc_trcEnd H3); intros.
+      econstructor; eauto.
+      unfold SYS; simpl.
+      econstructor; eauto.
+  Qed.
+
+  Lemma ss_implies_next_safe :
+    forall t (cmd : user_cmd t) uid ctx sty honestk cs froms sents,
+      syntactically_safe uid ctx cmd sty
+      -> typingcontext_sound ctx honestk cs uid
+      -> forall A B (usrs usrs' : honest_users A) (adv adv' : user_data B) cmd'
+          cs' gks gks' ks ks' qmsgs qmsgs' mycs mycs' froms' sents' n n' lbl,
+          step_user lbl (Some uid)
+                    (usrs,adv,cs,gks,ks,qmsgs,mycs,froms,sents,n,cmd)
+                    (usrs',adv',cs',gks',ks',qmsgs',mycs',froms',sents',n',cmd')
+          -> forall t__n (cmd__n : user_cmd t__n), nextAction cmd cmd__n
+          -> (forall r, cmd__n <> Return r)
+          -> no_resends sents'
+          -> next_cmd_safe honestk cs uid froms sents cmd.
+  Proof.
+    induct cmd;
+      unfold next_cmd_safe; intros;
+        match goal with
+        | [ H : nextAction _ _ |- _ ] => invert H
+        end; eauto;
+          try solve [ unfold typingcontext_sound in *; split_ex;
+                      match goal with
+                      | [ H : syntactically_safe _ _ _ _ |- _ ] => invert H
+                      end; eauto ].
+
+    - invert H0.
+      invert H2; eauto.
+      invert H3.
+      eapply IHcmd in H8; eauto.
+      eapply H8 in H10; eauto.
+
+      invert H3. invert H7. specialize (H4 a0); contradiction.
+
+    - unfold typingcontext_sound in *; split_ex; invert H.
+      apply H5 in H12; split_ex; subst.
+      apply H0 in H10.
+      unfold msg_honestly_signed, msg_signing_key,
+             msg_to_this_user, msg_destination_user,
+             msgCiphersSignedOk, honest_keyb;
+        context_map_rewrites.
+      destruct ( cipher_to_user x0 ==n cipher_to_user x0 ); try contradiction.
+      repeat simple apply conj; eauto.
+      econstructor; eauto.
+      unfold msg_honestly_signed, msg_signing_key, honest_keyb;
+        context_map_rewrites;
+        trivial.
+      (do 2 eexists); repeat simple apply conj; eauto.
+      invert H1.
+      unfold no_resends, updateSentNonce in H4; context_map_rewrites.
+      destruct (cipher_to_user x0 ==n cipher_to_user x0); try contradiction.
+      invert H4; eauto.
+      
+    - unfold typingcontext_sound in *; split_ex; invert H; eauto.
+      intros.
+      apply H14 in H; split_ex; subst; eauto.
+  Qed.
+
+  Lemma ss_implies_next_safe_not_send :
+    forall t (cmd : user_cmd t) uid ctx sty honestk cs froms sents,
+      syntactically_safe uid ctx cmd sty
+      -> typingcontext_sound ctx honestk cs uid
+      -> forall t__n (cmd__n : user_cmd t__n), nextAction cmd cmd__n
+      -> (forall t__msg recuid (msg : crypto t__msg), cmd__n ~= Send recuid msg -> False)
+      -> next_cmd_safe honestk cs uid froms sents cmd.
+  Proof.
+    induct cmd;
+      unfold next_cmd_safe; intros;
+        match goal with
+        | [ H : nextAction _ _ |- _ ] => invert H
+        end; eauto;
+          try solve [ unfold typingcontext_sound in *; split_ex;
+                      match goal with
+                      | [ H : syntactically_safe _ _ _ _ |- _ ] => invert H
+                      end; eauto ].
+
+    - invert H0.
+      invert H2; eauto.
+      eapply IHcmd in H11; eauto.
+      eapply na_deterministic in H8; eauto; split_ex; subst.
+      invert H2.
+      eapply H11 in H6; eauto.
+
+    - invert H1.
+      exfalso.
+      eapply H2; eauto.
+      
+    - unfold typingcontext_sound in *; split_ex; invert H; eauto.
+      intros.
+      apply H12 in H; split_ex; subst; eauto.
+
+      Unshelve.
+      eauto.
+  Qed.
+
+  Lemma ss_implies_next_safe_not_send' :
+    forall t (cmd : user_cmd t) uid ctx sty honestk cs froms sents,
+      syntactically_safe uid ctx cmd sty
+      -> typingcontext_sound ctx honestk cs uid
+      -> forall t__n (cmd__n : user_cmd t__n), nextAction cmd cmd__n
+      -> match cmd__n with
+        | Send recuid msg => t__n = Base Unit /\ (cmd__n ~= Send recuid msg -> False)
+        | _ => False
+        end
+      -> next_cmd_safe honestk cs uid froms sents cmd.
+  Proof.
+    induct cmd;
+      unfold next_cmd_safe; intros;
+        match goal with
+        | [ H : nextAction _ _ |- _ ] => invert H
+        end; eauto;
+          try solve [ unfold typingcontext_sound in *; split_ex;
+                      match goal with
+                      | [ H : syntactically_safe _ _ _ _ |- _ ] => invert H
+                      end; eauto ].
+
+    - invert H0.
+      invert H2; eauto.
+      eapply IHcmd in H11; eauto.
+      eapply na_deterministic in H8; eauto; split_ex; subst.
+      invert H2.
+      eapply H11 in H6; eauto.
+
+    - invert H1.
+      exfalso.
+      eapply H2; eauto.
+      
+    - unfold typingcontext_sound in *; split_ex; invert H; eauto.
+      intros.
+      apply H12 in H; split_ex; subst; eauto.
+
+      Unshelve.
+      eauto.
+  Qed.
+
+  (* Lemma ss_implies_next_safe_not_send : *)
+  (*   forall t__hon t__adv (usrs : honest_users t__hon)  (cmd : user_cmd t) uid ctx sty honestk cs froms sents, *)
+  (*     syntactically_safe uid ctx cmd sty *)
+  (*     -> typingcontext_sound ctx honestk cs uid *)
+  (*     -> forall t__n (cmd__n : user_cmd t__n), nextAction cmd cmd__n *)
+  (*     -> next_cmd_safe honestk cs uid froms sents cmd. *)
+  (* Proof. *)
+  (*   induct cmd; *)
+  (*     unfold next_cmd_safe; intros; *)
+  (*       match goal with *)
+  (*       | [ H : nextAction _ _ |- _ ] => invert H *)
+  (*       end; eauto; *)
+  (*         try solve [ unfold typingcontext_sound in *; split_ex; *)
+  (*                     match goal with *)
+  (*                     | [ H : syntactically_safe _ _ _ _ |- _ ] => invert H *)
+  (*                     end; eauto ]. *)
+
+  (*   - invert H0. *)
+  (*     invert H2; eauto. *)
+  (*     eapply IHcmd in H11; eauto. *)
+  (*     eapply na_deterministic in H8; eauto; split_ex; subst. *)
+  (*     invert H2. *)
+  (*     eapply H11 in H6; eauto. *)
+
+  (*   - invert H1. *)
+  (*     exfalso. *)
+  (*     eapply H2; eauto. *)
+      
+  (*   - unfold typingcontext_sound in *; split_ex; invert H; eauto. *)
+  (*     intros. *)
+  (*     apply H12 in H; split_ex; subst; eauto. *)
+
+  (*     Unshelve. *)
+  (*     eauto. *)
+  (* Qed. *)
+
+  
+
+  Lemma model_step_implies_step :
+    forall t__hon t__adv uid st st',
+      @model_step_user t__hon t__adv uid st st'
+      -> step st st'.
+  Proof.
+    intros * MS.
+    invert MS; intros.
+    - econstructor 1.
+      econstructor; eauto.
+    - econstructor 2; eauto.
+      econstructor; eauto.
+  Qed.
+
+  Import RealWorldNotations.
+
+  Lemma StepBindRecur' :
+    forall {B r r'} (usrs usrs' : honest_users r') (adv adv' : user_data B)
+      lbl u_id cs cs' qmsgs qmsgs' gks gks' ks ks' mycs mycs' froms froms' sents sents' cur_n cur_n'
+      (cmd1 cmd1' : user_cmd r) (cmd2 : <<r>> -> user_cmd (Base r')) bd bd',
+
+      step_user lbl u_id (usrs, adv, cs, gks, ks, qmsgs, mycs, froms, sents, cur_n, cmd1)
+                (usrs', adv', cs', gks', ks', qmsgs', mycs', froms', sents', cur_n', cmd1')
+      -> bd = (usrs, adv, cs, gks, ks, qmsgs, mycs, froms, sents, cur_n, Bind cmd1 cmd2)
+      -> bd' = (usrs', adv', cs', gks', ks', qmsgs', mycs', froms', sents', cur_n', Bind cmd1' cmd2)
+      -> forall lbl' suid',
+          lbl' = lbl
+          -> suid' = u_id
+          -> step_user lbl u_id bd bd'.
+  Proof.
+    intros; subst; eapply StepBindRecur; eauto.
+  Qed.
+
+  (* Lemma step_na_not_return : *)
+  (*   forall t t__n (cmd : user_cmd t) (cmd__n : user_cmd t__n), *)
+  (*     nextAction cmd cmd__n *)
+                 
+  (*     -> forall A B uid lbl bd bd' cs cs' (usrs usrs': honest_users A) (adv adv' : user_data B) gks gks' *)
+  (*         cmd__n' ks ks' qmsgs qmsgs' mycs mycs' *)
+  (*         froms froms' sents sents' cur_n cur_n' , *)
+
+  (*       step_user lbl (Some uid) bd bd' *)
+  (*       -> bd = (usrs, adv, cs, gks, ks, qmsgs, mycs, froms, sents, cur_n, cmd__n) *)
+  (*       -> bd' = (usrs', adv', cs', gks', ks', qmsgs', mycs', froms', sents', cur_n', cmd__n') *)
+  (*       -> exists f cmd', *)
+  (*           cmd = f cmd__n *)
+  (*           /\ cmd' = f cmd__n' *)
+  (*           /\ forall lbl1 suid1 (usrs1 usrs1' : honest_users A) (adv1 adv1' : user_data B) *)
+  (*               cs1 cs1' gks1 gks1' *)
+  (*               ks1 ks1' qmsgs1 qmsgs1' mycs1 mycs1' cmd__n'' *)
+  (*               froms1 froms1' sents1 sents1' cur_n1 cur_n1', *)
+
+  (*               step_user lbl1 suid1 *)
+  (*                         (usrs1, adv1, cs1, gks1, ks1, qmsgs1, mycs1, froms1, sents1, cur_n1, cmd__n) *)
+  (*                         (usrs1', adv1', cs1', gks1', ks1', qmsgs1', mycs1', froms1', sents1', cur_n1', cmd__n'') *)
+  (*               -> step_user lbl1 suid1 *)
+  (*                           (usrs1, adv1, cs1, gks1, ks1, qmsgs1, mycs1, froms1, sents1, cur_n1, f cmd__n) *)
+  (*                           (usrs1', adv1', cs1', gks1', ks1', qmsgs1', mycs1', froms1', sents1', cur_n1', f cmd__n''). *)
+  (* Proof. *)
+  (*   induction 1; inversion 2; inversion 1; intros; subst. *)
+  (*   - invert H. *)
+  (*   - exists (fun x => x); eexists; repeat simple apply conj; eauto. *)
+  (*   - exists (fun x => x); eexists; repeat simple apply conj; eauto. *)
+  (*   - exists (fun x => x); eexists; repeat simple apply conj; eauto. *)
+  (*   - exists (fun x => x); eexists; repeat simple apply conj; eauto. *)
+  (*   - exists (fun x => x); eexists; repeat simple apply conj; eauto. *)
+  (*   - exists (fun x => x); eexists; repeat simple apply conj; eauto. *)
+  (*   - exists (fun x => x); eexists; repeat simple apply conj; eauto. *)
+  (*   - exists (fun x => x); eexists; repeat simple apply conj; eauto. *)
+  (*   - exists (fun x => x); eexists; repeat simple apply conj; eauto. *)
+  (*   - clean_context. *)
+  (*     eapply IHnextAction in H0; eauto; split_ex; subst. *)
+  (*     exists (fun CD => x <- x CD; c2 x). *)
+  (*     eexists; subst; repeat simple apply conj; intros; eauto. *)
+  (*     eapply StepBindRecur'. *)
+  (*     remember (Some uid) as suid. *)
+  (*     match goal with *)
+  (*     | [ |- step_user _ _ ?bd1 ?bd2 ] => *)
+  (*       remember bd1 as bbd1; *)
+  (*         remember bd2 as bbd2 *)
+  (*     end. *)
+
+  
+  (* Lemma step_na_not_return : *)
+  (*   forall t t__n (cmd : user_cmd t) (cmd__n : user_cmd t__n), *)
+  (*     nextAction cmd cmd__n *)
+                 
+  (*     -> forall A B uid lbl bd bd' cs cs' (usrs usrs': honest_users A) (adv adv' : user_data B) gks gks' *)
+  (*         cmd__n' ks ks' qmsgs qmsgs' mycs mycs' *)
+  (*         froms froms' sents sents' cur_n cur_n' , *)
+
+  (*       step_user lbl (Some uid) bd bd' *)
+  (*       -> bd = (usrs, adv, cs, gks, ks, qmsgs, mycs, froms, sents, cur_n, cmd__n) *)
+  (*       -> bd' = (usrs', adv', cs', gks', ks', qmsgs', mycs', froms', sents', cur_n', cmd__n') *)
+  (*       -> exists f cmd', *)
+  (*           cmd = f cmd__n *)
+  (*           /\ cmd' = f cmd__n' *)
+  (*           /\ step_user lbl (Some uid) *)
+  (*                       (usrs, adv, cs, gks, ks, qmsgs, mycs, froms, sents, cur_n, f cmd__n) *)
+  (*                       (usrs', adv', cs', gks', ks', qmsgs', mycs', froms', sents', cur_n', f cmd__n'). *)
+  (* Proof. *)
+  (*   induction 1; inversion 2; inversion 1; intros; subst. *)
+  (*   - invert H. *)
+  (*   - exists (fun x => x); eexists; repeat simple apply conj; eauto. *)
+  (*   - exists (fun x => x); eexists; repeat simple apply conj; eauto. *)
+  (*   - exists (fun x => x); eexists; repeat simple apply conj; eauto. *)
+  (*   - exists (fun x => x); eexists; repeat simple apply conj; eauto. *)
+  (*   - exists (fun x => x); eexists; repeat simple apply conj; eauto. *)
+  (*   - exists (fun x => x); eexists; repeat simple apply conj; eauto. *)
+  (*   - exists (fun x => x); eexists; repeat simple apply conj; eauto. *)
+  (*   - exists (fun x => x); eexists; repeat simple apply conj; eauto. *)
+  (*   - exists (fun x => x); eexists; repeat simple apply conj; eauto. *)
+  (*   - clean_context. *)
+  (*     eapply IHnextAction in H0; eauto; split_ex; subst. *)
+  (*     exists (fun CD => x <- x CD; c2 x). *)
+  (*     eexists; subst; repeat simple apply conj; eauto. *)
+  (*     eapply StepBindRecur'. *)
+  (*     remember (Some uid) as suid. *)
+  (*     match goal with *)
+  (*     | [ |- step_user _ _ ?bd1 ?bd2 ] => *)
+  (*       remember bd1 as bbd1; *)
+  (*         remember bd2 as bbd2 *)
+  (*     end. *)
+
+      
+  (*     eapply StepBindRecur' with (cmd1 := x c) (cmd1' :=  x cmd__n') (cmd2 := c2). *)
+    
+
+
+  (* Lemma step_na_not_return : *)
+  (*   forall {A B C} suid lbl bd bd', *)
+
+  (*     step_user lbl suid bd bd' *)
+
+  (*     -> forall cs cs' (usrs usrs': honest_users A) (adv adv' : user_data B) gks gks' *)
+  (*         (cmd__n cmd__n' : user_cmd C) (cmd : user_cmd (Base A)) ks ks' qmsgs qmsgs' mycs mycs' *)
+  (*         froms froms' sents sents' cur_n cur_n', *)
+
+  (*       bd = (usrs, adv, cs, gks, ks, qmsgs, mycs, froms, sents, cur_n, cmd__n) *)
+  (*       -> bd' = (usrs', adv', cs', gks', ks', qmsgs', mycs', froms', sents', cur_n', cmd__n') *)
+  (*       -> nextAction cmd cmd__n *)
+  (*       -> exists f cmd', *)
+  (*           (* step_user lbl suid *) *)
+  (*           (*           (usrs, adv, cs, gks, ks, qmsgs, mycs, froms, sents, cur_n, cmd__n) *) *)
+  (*           (*           (usrs', adv', cs', gks', ks', qmsgs', mycs', froms', sents', cur_n', cmd__n') *) *)
+  (*             cmd = f cmd__n *)
+  (*           /\ cmd' = f cmd__n' *)
+  (*           /\ step_user lbl suid *)
+  (*                       (usrs, adv, cs, gks, ks, qmsgs, mycs, froms, sents, cur_n, f cmd__n) *)
+  (*                       (usrs', adv', cs', gks', ks', qmsgs', mycs', froms', sents', cur_n', f cmd__n'). *)
+  (* Proof. *)
+  (*   Hint Constructors step_user syntactically_safe : core. *)
+
+  (*   induction 1; inversion 1; inversion 1; intros; subst. *)
+
+  (*   - eapply nextAction_couldBe in H13; contradiction. *)
+  (*   - eapply nextAction_couldBe in H12; contradiction. *)
+  (*   -  *)
+
+
+  (*   - eapply IHstep_user in H28; eauto. *)
+  (*     split_ex. *)
+  (*     exists (fun CD => x <- x CD; cmd2 x). *)
+  (*     eexists; subst; repeat simple apply conj; eauto. *)
+      
+  (*   - invert H27. *)
+  (*     unfold not in *; exfalso; eauto. *)
+  (*   - exists (fun x => x); eexists; repeat simple apply conj; swap 1 3; eauto. *)
+  (*   - exists (fun x => x); eexists; repeat simple apply conj; swap 1 3; eauto. *)
+  (*   - exists (fun x => x); eexists; repeat simple apply conj; swap 1 3; eauto. *)
+  (*   - exists (fun x => x); eexists; repeat simple apply conj; swap 1 3; eauto. *)
+  (*   - exists (fun x => x); eexists; repeat simple apply conj; swap 1 3; eauto. *)
+  (*   - exists (fun x => x); eexists; repeat simple apply conj; swap 1 3; eauto. *)
+  (*   - exists (fun x => x); eexists; repeat simple apply conj; swap 1 3; eauto. *)
+  (*   - exists (fun x => x); eexists; repeat simple apply conj; swap 1 3; eauto. *)
+  (*   - exists (fun x => x); eexists; repeat simple apply conj; swap 1 3; eauto. *)
+  (*   - exists (fun x => x); eexists; repeat simple apply conj; swap 1 3; eauto. *)
+  (* Qed. *)
+
+
+  Lemma simsafe : honest_actions_safe t__adv R.
+  Proof.
+    hnf
+    ; intros * REL UOK AUOK
+    ; invert REL.
+
+    pose proof no_resends_inv.
+    unfold invariantFor, SYS in H0; simpl in H0.
+    assert ( (ru0,iu0) = (ru0,iu0) \/ False ) as ARG by auto.
+    specialize (H0 _ ARG).
+
+    assert (syntactically_safe_U ru) by admit.
+    unfold syntactically_safe_U in *; simpl in *.
+    unfold honest_cmds_safe; intros; subst.
+    destruct u; simpl.
+    generalize H6; intros USRS; rewrite <- H in USRS.
+    specialize (H4 _ _ USRS); split_ex; simpl in *.
+
+    rename U__i into iu.
+    red. intros.
+
+    destruct (classic (exists st', model_step_user u_id (ru,iu) st')).
+    - split_ex.
+      rename x1 into st'.
+      pose proof (model_step_implies_step _ _ _ _ _ H8) as STEP.
+      assert (STEPS' : (@step t__hon t__adv) ^* (ru,iu) st') by (eauto using TrcFront).
+      pose proof (trc_trans H3 STEPS') as STEPS.
+
+      specialize (H0 _ STEPS); unfold no_resends_U in H0.
+      destruct st' as [ru1 iu1]; simpl in *.
+
+      rewrite <- H, <- H1.
+      destruct (classic (exists r, cmd__n = Return r)); split_ex; subst; eauto.
+      assert (forall r, cmd__n <> Return r) by eauto using all_not_not_ex.
+
+      rewrite Forall_natmap_forall in H0.
+      
+      destruct ru; invert H8;
+        unfold build_data_step in *;
+        clean_map_lookups;
+        simpl in *;
+        eapply ss_implies_next_safe; eauto.
+
+      specialize (H0 u_id); rewrite add_eq_o in H0 by trivial;
+        specialize (H0 _ eq_refl);
+        eauto.
+
+      specialize (H0 u_id); rewrite add_eq_o in H0 by trivial;
+        specialize (H0 _ eq_refl);
+        eauto.
+
+    - dependent destruction cmd__n; eauto.
+      + eapply nextAction_couldBe in H7; contradiction.
+      + exfalso.
+        assert (forall st', model_step_user u_id (ru,iu) st' -> False) by eauto using not_ex_all_not.
+        pose proof stuck_not_misaligned_inv as NOTMISAL.
+        specialize (NOTMISAL _ ARG _ H3).
+        eapply NOTMISAL in H9.
+        2: simpl; exact USRS.
+
+        
+        unfold build_data_step in *; simpl in *.
+        assert (STEP : exists lbl bd,
+                   step_user lbl
+                             (Some u_id)
+                             (users ru, adversary ru, all_ciphers ru, all_keys ru,
+                              key_heap, msg_heap, c_heap, from_nons, sent_nons, cur_nonce, Send uid msg) bd).
+        (do 2 eexists).
+        econstructor; eauto.
+
+        unfold typingcontext_sound in *.
+        
+
+        
+        eapply step_na_not_return in H7; eauto.
+        
+        eapply H9.
+        unfold build_data_step; simpl.
+
+        
+
+
+    - destruct (classic (forall t__msg recuid (msg : crypto t__msg), cmd__n ~= Send recuid msg -> False)).
+      + eapply ss_implies_next_safe_not_send; eauto.
+        rewrite <- H, <- H1; assumption.
+      + dependent destruction cmd__n; eauto.
+
+      
+
+    - destruct (classic (match cmd__n with
+                         | Send recuid msg => B = Base Unit /\ (cmd__n ~= Send recuid msg -> False)
+                         | _ => False
+                         end)).
+
+      + eapply ss_implies_next_safe_not_send; eauto.
+        rewrite <- H, <- H1; assumption.
+        dependent destruction cmd__n; try contradiction.
+        split_ands; eauto.
+
+      + dependent destruction cmd__n; eauto.
+        * eapply nextAction_couldBe in H7; contradiction.
+        * exfalso.
+          eapply H9.
+          split; intros; eauto.
+          invert
+        
+        
+
+
+      
+    - destruct (classic (forall t__msg recuid (msg : crypto t__msg), cmd__n ~= Send recuid msg -> False)).
+      + eapply ss_implies_next_safe_not_send; eauto.
+        rewrite <- H, <- H1; assumption.
+
+      + exfalso.
+        eapply H9.
+        intros.
+        invert H10.
+
+        
+        
+      
+
+      dependent destruction cmd__n; auto.
+      apply nextAction_couldBe in H7; contradiction.
+      eapply ss_implies_next_safe in H7; eauto.
+
+      
+      (* rewrite Forall_natmap_forall in H0; *)
+      (*   specialize (H0 _ _ USRS). *)
+      (* invert H8; simpl in *. *)
+      (* eapply ss_implies_next_safe; eauto. *)
+      (* unfold next_cmd_safe; intros. *)
+
+      (* induct H8; eauto. *)
+      (* admit. *)
+      (* invert H4. *)
+      (* eapply IHnextAction in H15; eauto. *)
+      
+
+      (* generalize H8; intros NA; apply nextAction_couldBe in NA. *)
+      (* dependent destruction protocol; try contradiction; eauto. *)
+      admit.
+
+    - 
+
+
+
+      
+      (* rewrite Forall_natmap_forall in H0; specialize (H0 _ _ USRS); simpl in H0. *)
+      (* eapply predicates_imply_next_cmd_safe; eauto. *)
+      admit.
+    - admit.
+
+
+    (* pose proof safety_inv. *)
+    (* unfold invariantFor, SYS in H0; simpl in H0. *)
+    (* assert ( (ru0,iu0) = (ru0,iu0) \/ False ) as ARG by eauto. *)
+    (* specialize (H0 _ ARG _ H3). *)
+    (* unfold safety in *; eauto with safe. *)
+
   Admitted.
+
+  Hint Resolve simsilent simlabeled simsafe : safe.
+
+  Lemma proto_lamely_refines :
+    refines (lameAdv b) ru0 iu0.
+  Proof.
+    exists R; unfold simulates.
+
+    pose proof safe_invariant.
+    pose proof universe_starts_safe; split_ands.
+    
+    unfold invariantFor in H; simpl in H.
+    assert ( (ru0,iu0) = (ru0,iu0) \/ False ) as ARG by eauto.
+    specialize (H _ ARG); clear ARG.
+
+    Hint Constructors R : safe.
+
+    unfold simulates_silent_step, simulates_labeled_step;
+      intuition eauto with safe.
+
+  Qed.
+
+  Hint Resolve proto_lamely_refines : safe.
+
+  Lemma proto_starts_ok : universe_starts_ok ru0.
+  Proof.
+    pose proof universe_starts_safe.
+    pose proof U_good.
+    unfold universe_starts_ok; intros.
+    unfold universe_ok, adv_universe_ok, universe_starts_sane in *; split_ands.
+    intuition eauto.
+  Qed.
+
+  Hint Resolve proto_starts_ok : safe.
+
+  Theorem protocol_with_adversary_could_generate_spec :
+    forall U__ra advcode acts__r,
+      U__ra = add_adversary ru0 advcode
+      -> rCouldGenerate U__ra acts__r
+      -> exists acts__i,
+          iCouldGenerate iu0 acts__i
+          /\ traceMatches acts__r acts__i.
+  Proof.
+    intros.
+    pose proof U_good as L; unfold universe_starts_sane, adversary_is_lame in L; split_ands.
+    eapply refines_could_generate; eauto with safe.
+  Qed.
+
+End ProtocolSimulates.
+
 
   (* Lemma honest_cmds_safe_adv_change : *)
   (*   forall {t1 t2} (U U' : RealWorld.universe t1 t2), *)
@@ -568,20 +1108,17 @@ Module ProtocolSimulates (Proto : SyntacticallySafeProtocol).
 
   (* Hint Resolve honest_cmds_safe_adv_change : safe. *)
 
-  Require Import Coq.Program.Equality.
+  (* Lemma foo : *)
+  (*   forall A B t (cmd : user_cmd t) (usrs : honest_users A) (adv : user_data B) cs gks *)
+  (*     uid ks qmsgs mycs froms sents n, *)
+  (*       (forall lbl bd, ~ step_user lbl (Some uid) (usrs,adv,cs,gks,ks,qmsgs,mycs,froms,sents,n,cmd) bd) *)
+  (*       -> forall t__n cmd1 (cmd2 : <<t__n>> -> user_cmd t), *)
+  (*       cmd = Bind cmd1 cmd2 *)
+  (*       -> forall lbl' bd', *)
+  (*         ~ step_user lbl' (Some uid) (usrs,adv,cs,gks,ks,qmsgs,mycs,froms,sents,n,cmd1) bd'. *)
+  (* Admitted. *)
 
-  Lemma foo :
-    forall A B t (cmd : user_cmd t) (usrs : honest_users A) (adv : user_data B) cs gks
-      uid ks qmsgs mycs froms sents n,
-        (forall lbl bd, ~ step_user lbl (Some uid) (usrs,adv,cs,gks,ks,qmsgs,mycs,froms,sents,n,cmd) bd)
-        -> forall t__n cmd1 (cmd2 : <<t__n>> -> user_cmd t),
-        cmd = Bind cmd1 cmd2
-        -> forall lbl' bd',
-          ~ step_user lbl' (Some uid) (usrs,adv,cs,gks,ks,qmsgs,mycs,froms,sents,n,cmd1) bd'.
-  Admitted.
-
-  Hint Resolve foo : core.
-    
+  (* Hint Resolve foo : core. *)
 
   (* Lemma predicates_imply_next_cmd_safe_no_step' : *)
   (*   forall A B t (cmd : user_cmd t) (usrs : honest_users A) (adv : user_data B) cs gks *)
@@ -690,95 +1227,4 @@ Module ProtocolSimulates (Proto : SyntacticallySafeProtocol).
   (*   - intros. *)
   (*     eapply H14 in H5; split_ex; subst; split; eauto. *)
   (* Qed. *)
-  
-      
-  Lemma simsafe : honest_actions_safe t__adv R.
-  Proof.
-    hnf
-    ; intros * REL UOK AUOK
-    ; invert REL.
-
-    pose proof no_resends_inv.
-    unfold invariantFor, SYS in H0; simpl in H0.
-    assert ( (ru0,iu0) = (ru0,iu0) \/ False ) as ARG by auto.
-    specialize (H0 _ ARG); clear ARG.
-
-    assert (syntactically_safe_U ru) by admit.
-    unfold syntactically_safe_U in *; simpl in *.
-    unfold honest_cmds_safe; intros; subst.
-    destruct u; simpl.
-    generalize H6; intros USRS; rewrite <- H in USRS.
-    specialize (H4 _ _ USRS); split_ex; simpl in *.
-
-    rename U__i into iu.
-    destruct (classic (exists st', step (ru,iu) st')).
-    - split_ex.
-      rename x1 into st'.
-      assert (STEP : (@step t__hon t__adv) ^* (ru,iu) st') by (eauto using TrcFront).
-      pose proof (trc_trans H3 STEP) as STEPS.
-
-      specialize (H0 _ STEPS); unfold no_resends_U in H0.
-      
-      (* rewrite Forall_natmap_forall in H0; specialize (H0 _ _ USRS); simpl in H0. *)
-      (* eapply predicates_imply_next_cmd_safe; eauto. *)
-      admit.
-    - admit.
-
-
-    (* pose proof safety_inv. *)
-    (* unfold invariantFor, SYS in H0; simpl in H0. *)
-    (* assert ( (ru0,iu0) = (ru0,iu0) \/ False ) as ARG by eauto. *)
-    (* specialize (H0 _ ARG _ H3). *)
-    (* unfold safety in *; eauto with safe. *)
-
-  Admitted.
-
-  Hint Resolve simsilent simlabeled simsafe : safe.
-
-  Lemma proto_lamely_refines :
-    refines (lameAdv b) ru0 iu0.
-  Proof.
-    exists R; unfold simulates.
-
-    pose proof safe_invariant.
-    pose proof universe_starts_safe; split_ands.
-    
-    unfold invariantFor in H; simpl in H.
-    assert ( (ru0,iu0) = (ru0,iu0) \/ False ) as ARG by eauto.
-    specialize (H _ ARG); clear ARG.
-
-    Hint Constructors R : safe.
-
-    unfold simulates_silent_step, simulates_labeled_step;
-      intuition eauto with safe.
-
-  Qed.
-
-  Hint Resolve proto_lamely_refines : safe.
-
-  Lemma proto_starts_ok : universe_starts_ok ru0.
-  Proof.
-    pose proof universe_starts_safe.
-    pose proof U_good.
-    unfold universe_starts_ok; intros.
-    unfold universe_ok, adv_universe_ok, universe_starts_sane in *; split_ands.
-    intuition eauto.
-  Qed.
-
-  Hint Resolve proto_starts_ok : safe.
-
-  Theorem protocol_with_adversary_could_generate_spec :
-    forall U__ra advcode acts__r,
-      U__ra = add_adversary ru0 advcode
-      -> rCouldGenerate U__ra acts__r
-      -> exists acts__i,
-          iCouldGenerate iu0 acts__i
-          /\ traceMatches acts__r acts__i.
-  Proof.
-    intros.
-    pose proof U_good as L; unfold universe_starts_sane, adversary_is_lame in L; split_ands.
-    eapply refines_could_generate; eauto with safe.
-  Qed.
-
-End ProtocolSimulates.
 
